Phi_System/IDE_CP_App2.thy
@@ -342,9 +342,7 @@ subsubsection \<open>Semantic Zero Value\<close>
 context begin
 
 private lemma \<phi>TA_Semantic_Zero_Val_rule:
-  \<open> \<c>\<o>\<n>\<d>\<i>\<t>\<i>\<o>\<n> Zero TY = Some v
-\<Longrightarrow> \<r>Success
-\<Longrightarrow> Ant \<longrightarrow> (\<c>\<o>\<n>\<d>\<i>\<t>\<i>\<o>\<n> v \<Turnstile> (z \<Ztypecolon> T))
+  \<open> (Ant \<Longrightarrow> \<p>\<r>\<e>\<m>\<i>\<s>\<e> Zero TY \<noteq> None \<and> (\<forall>v. Zero TY = Some v \<longrightarrow> v \<Turnstile> (z \<Ztypecolon> T)))
 \<Longrightarrow> \<r>Success
 \<Longrightarrow> \<o>\<b>\<l>\<i>\<g>\<a>\<t>\<i>\<o>\<n> True
 \<Longrightarrow> Ant @action \<phi>TA_ANT
